LambdaS5/caml/ljs/ljs_pretty.ml
@@ -32,6 +32,7 @@ let string_of_unary_op s = match s with
     | Coq_unary_op_strlen -> "strlen"
     | Coq_unary_op_to_int32 -> "to-int32"
     | Coq_unary_op_not -> "!"
+    | Coq_unary_op_neg -> "-"
     | Coq_unary_op_floor -> "floor"
     | Coq_unary_op_ceil -> "ceil"
     | Coq_unary_op_abs -> "abs"
